update

Bridge.ml
@@ -2,18 +2,14 @@ type ('ok , 'error) result = ('ok , 'error) Base.result =
   | Ok of 'ok
   | Error of 'error
 
-(* OCaml doesn't have official unsined int. *)
 let native_int_bits = Z.of_int (Sys.int_size + 1)
-let native_uint_bits = Z.of_int Sys.int_size
 
 type native_int = int
-type native_uint = int
 
 type isize = Z.t
-type usize = Z.t
 
 let of_int = Z.of_int
-let of_uint = Z.of_int
 
 let to_native_int _ = Z.to_int
-let to_native_uint _ = Z.to_int
+
+type 'a native_list = 'a list
