Bridge.fsti
@@ -12,19 +12,14 @@ val native_int_bits: Prims.pos
 val native_uint_bits: Prims.pos
 
 assume new type native_int
-assume new type native_uint
 
 type isize = I.int_t native_int_bits
-type usize = UI.uint_t native_uint_bits
 
 val of_int: native_int -> Tot isize
-val of_uint: native_uint -> Tot usize
 
 val to_native_int:
     #s:pos
     -> (n:I.int_t s{s <= native_int_bits})
     -> Tot (native_n:native_int{of_int native_n = n})
-val to_native_uint:
-    #s:pos
-    -> (n:UI.uint_t s{s <= native_uint_bits})
-    -> Tot (native_n:native_uint{of_uint native_n = n})
+
+type native_list 'a = (l:list 'a{L.length l <= I.max_int native_int_bits})
