hamming/Hamming.fst
@@ -8,10 +8,10 @@ module L = FStar.List.Pure
 type nucleotide = | A | C | G | T
 
 (** Compute the hamming distance between the two lists. *)
-val hamming_distance : (l1: list nucleotide) -> (l2: list nucleotide) -> Tot (res: result native_uint string{
+val hamming_distance : (l1: native_list nucleotide) -> (l2: native_list nucleotide) -> Tot (res: result native_int string{
         match res with
             | Ok distance -> L.length l1 = L.length l2
-                            /\ 0 <= of_uint distance /\ of_uint distance <= L.length l1
+                            /\ 0 <= of_int distance /\ of_int distance <= L.length l1
             | Error msg -> msg = "left strand must not be empty"
                         \/ msg = "right strand must not be empty"
                         \/ msg = "left and right strands must be of equal length"
@@ -20,4 +20,4 @@ let hamming_distance l1 l2 = match l1, l2 with
     | l1, l2 when L.length l1 <> L.length l2 && L.length l1 = 0  -> Error "left strand must not be empty"
     | l1, l2 when L.length l1 <> L.length l2 && L.length l2 = 0 -> Error "right strand must not be empty"
     | l1, l2 when L.length l1 <> L.length l2 -> Error "left and right strands must be of equal length"
-    | l1, l2 -> Ok (to_native_uint #native_uint_bits (L.length (L.filter (fun (e1, e2) -> e1 <> e2) (L.zip l1 l2))))
+    | l1, l2 -> Ok (to_native_int #native_int_bits (L.length (L.filter (fun (e1, e2) -> e1 <> e2) (L.zip l1 l2))))
